\documentclass[a4paper,12pt]{article}
\usepackage[ukrainian,english]{babel}
\usepackage{ucs}
\usepackage[utf8]{inputenc}
\usepackage[T2A]{fontenc}
\usepackage{amsmath}
\usepackage{bigints}
\usepackage{amsfonts}
\usepackage{graphicx}
\newcommand{\dx}{\textbf{d}x}
\newcommand{\dt}{\textbf{d}t}
\newcommand{\dy}{\textbf{d}}
\newcommand{\arch}{\textrm{arcch}}
\newcommand{\arsh}{\textrm{arcsh}}
\newcommand\tab[1][1cm]{\hspace*{#1}}
\usepackage[left=20mm, top=20mm, right=10mm, bottom=20mm, nohead, nofoot]{geometry}
\begin{document}
\begin{center}
{\LARGE Домашня робота 4}	
\end{center}
\begin{itemize}
	\item [3.15] $\bigintsss\frac{2x+3}{(x-2)(x+5)}\dx=\frac27\bigintsss\frac{\dx}{x-2}+\frac57\bigintsss\frac{\dx}{x+5}=\frac27\ln|x-2|+\frac57\ln|x+5|+c$
	\item [3.16] $\bigintsss\frac{x^3+1}{x^3-5x^2+6x}\dx=\frac16\bigintsss\frac{\dx}{x}-\frac92\bigintsss\frac{\dx}{x-2}+\frac{28}3\bigintsss\frac{\dx}{x-3}=\frac16\ln|x|-\frac92\ln|x-2|+\frac{28}3\ln|x-3|+c$
	\item [3.17] $\bigintsss\frac{\dx}{(x+1)(x^2+1)}=\frac12\bigintsss\frac{\dx}{x+1}-\frac12\bigintsss\frac{x-1}{x^2+1}\dx=\\=\frac12\left(\ln|x+1|-\bigintsss\frac{x}{x^2+1}\dx\left|u=x^2+1\>\>\dx=\frac1{2x}\dy u \right|+\bigintsss\frac{\dx}{x^2+1} \right)=\\=\frac12\left(\ln|x+1|+\frac12\ln|x^2+1|+\arctan x \right)+c$
	\item [3.18] $\bigintsss\frac{\dx}{x(x+1)(x^2+x+1)}=\bigintsss\frac{\dx}{x}-\bigintsss\frac{\dx}{x+1}-\bigintsss\frac{\dx}{x^2+x+1}=\ln|x|-\ln|x+1|-\\-\bigintsss\frac{\dx}{(x+0.5)^2+0.75}\left|u=\frac{2x+1}{\sqrt3}\right|=\ln|x|-\ln|x+1|-\frac2{\sqrt3}\ln\left|\frac{2x+1}{\sqrt3}\right|+c$
\end{itemize}






















\end{document}