\documentclass[a4paper,12pt]{article}
\usepackage[none]{hyphenat}
\usepackage[russian,english]{babel}
\usepackage{ucs}
\usepackage[utf8]{inputenc}
\usepackage[T2A]{fontenc}
\usepackage{graphicx}
\usepackage{wrapfig}
\usepackage{amsfonts}
\usepackage{amsthm}
\usepackage{amssymb}
\usepackage{amsmath}
\usepackage{mdframed} 
\usepackage{xcolor}
\usepackage{xparse} 
\usepackage{scalerel}
\usepackage{stackengine}
\usepackage{bigints}
\usepackage{enumerate}	
\usepackage{mathtools}
\usepackage{multicol}
\usepackage{longdivision}
\usepackage{polynom}
\usepackage{cancel}
\usepackage{extarrows}
\usepackage{ragged2e}
\newcommand\showdiv[1]{\overline{\smash{\hstretch{.5}{\right)}\mkern-3.2mu\hstretch{.5}{\right)}}#1}}
\let\ph\phantom
\newcommand\tab[1][1cm]{\hspace*{#1}}
\newcommand\dx{\textbf{ d}x}
\newcommand\dt{\textbf{ d}t}
\newcommand\dint{\displaystyle\int\limits}
\newcommand\dsum{\displaystyle\sum\limits^\infty}
\newcommand{\limm}{\lim\limits_{n\to\infty}}
\newcommand\dy{\textbf{ d}}
\newcommand\const{\textrm{const}}
\newcommand\lcm{\textrm{lcm}}
\newcommand{\longeq}{\scalebox{2}[1]{=}}
\newcommand{\zstroke}{%
  \text{\ooalign{\hidewidth -\kern-.3em-\hidewidth\cr$z$\cr}}%
}
\usepackage[left=20mm, top=20mm, right=10mm, bottom=20mm, nohead, nofoot]{geometry}
\begin{document}
	\begin{enumerate}
		\item \begin{enumerate} 
			\item $\dsum_{n=1}\left(\dfrac{2n}{4n+3}\right)^{n^2}\\\limm\sqrt[n]{a_n}=\limm\sqrt[n]{\left(\dfrac{2n}{4n+3}\right)^{n^2}}=\limm\left(\dfrac{2n}{4n+3}\right)^{n}=\limm\left(\dfrac{2}{4+\frac3n}\right)^{n}=\limm\dfrac1{2^n}=0<1\\\Rightarrow$ ряд збіжний
			\item $\dsum_{n=4}\dfrac{n+1}{(5n^2-9)\ln(n-2)}\\\dint_4^\infty\dfrac{\dx}{(x-2)\ln(x-2)}=\lim\limits_{b\to\infty}\dint_4^b\dfrac{\dx}{(x-2)\ln(x-2)}=|t=\ln(x-2)|=\lim\limits_{b\to\infty}\dint_{\ln2}^{\ln(b-2)}\dfrac{\dt}{t}=\\=\lim\limits_{b\to\infty}\ln|t|\Bigg|_{\ln2}^{\ln(b-2)}=\lim\limits_{b\to\infty}\ln\ln\left(\dfrac b2-1\right)=\infty\Rightarrow$ ряд розбіжний
			\item $\dsum_{n=1}\dfrac{n^2}{\sqrt{n^7+4n^2+5}}\\\limm\left(\dfrac{\dfrac{n^2}{\sqrt{n^7+4n^2+5}}}{\dfrac1{n^{\frac23}}}\right)=\limm\left(\dfrac{n^\frac72}{\sqrt{n^7+4n^2+5}}\right)=\limm\left(\dfrac1{\sqrt{1+\frac4{n^5}+\frac5{n^7}}}\right)=1\\\Rightarrow$ ряд збіжний
			\item $\dsum_{n=1}\dfrac{3n^2+2n+\ln n}{n^5+ne^n+3n}\\\limm\dfrac{\dfrac{3(n+1)^2+2(n+1)+\ln(n+1)}{(n+1)^5+(n+1)e^(n+1)+3(n+1)}}{\dfrac{3n^2+2n+\ln n}{n^5+ne^n+3n}}=\dfrac1e\\\Rightarrow$ ряд збіжний
			\item $\dsum_{n=1}\sqrt{n}\left(1-\cos\dfrac1n\right)$\begin{flalign*}
				n\to\infty:\tab&\sqrt{n}\to\infty&\\&\dfrac1n\to0\\&\cos\dfrac1n\to1\\&\sqrt{n}\left(1-\cos\dfrac1n\right)\to\textrm{невизначено}
			\end{flalign*}$\Rightarrow$ ряд розбіжний
		\end{enumerate}
		\item $\dsum_{n=1}(-1)^n\dfrac{\sin3^n}{3^n},\dsum_{n=1}\dfrac{|\sin3^n|}{3^n}\\\dsum_{n=1}\dfrac{1}{3^n}$ - збіжний при $q=\dfrac13<1,|\sin3^n|\leq1\Rightarrow\dfrac{|\sin3^n|}{3^n}\leq\dfrac1{3^n}\Rightarrow\dsum_{n=1}\dfrac{|\sin3^n|}{3^n}$  - збіжний\\$\Rightarrow\dsum_{n=1}(-1)^n\dfrac{\sin3^n}{3^n}$ -  також збіжний
		\item $\dsum_{n=1}\dfrac{(-1)^n}{(4n-1)2^n}(x+2)^n=\dsum_{n=1}a_nt^n,a_n=\dfrac{(-1)^n}{4n-1},t=\dfrac{x+2}2\\a_{n+1}=\dfrac{(-1)^{n+1}}{4n},\limm\left|\dfrac{\dfrac{(-1)^{n+1}}{4n}}{\dfrac{(-1)^n}{4n-1}} \right|=\limm\left|-\dfrac{4n-1}{4n} \right|=\limm\left|-\dfrac{4-\frac1n}{4} \right|=1\Rightarrow t\in(-1,1)\\t=1:\dsum_{n=1}\dfrac{(-1)^n}{4n-1}$ - збіжний, $t=-1:\dsum_{n=1}-\dfrac{(-1)^n}{4n-1}$ - умовно збіжний $\Rightarrow t\in[-1,1)\\-1<\left(\dfrac{x+2}2\right)\leq1\Rightarrow x\in(-4,0]\\$Область збіжності: $x\in[-4,0]$
		\item $f(x)=1+\cos3x\\\tab f'(x)=-3\sin3x\\\tab f''(x)=-9\cos3x\\\tab f'''(x)=27\sin3x\\\tab f^{IV}(x)=81\cos3x\\f(x)=1+\cos3x=2+0+\dfrac{-9}2x^2+0+\dfrac{81}{8}x^4+\dots=2-\dfrac92x^2+\dfrac{81}8x^4+\dots$
		\item \begin{enumerate} 
			\item $\dsum_{n=1}\dfrac{(-1)^nn}{n^2+15}\\\limm\dfrac{a_{n+1}}{a_n}=\limm\dfrac{\dfrac{(-1)^{n+1}(n+1)}{(n+1)^2+15}}{\dfrac{(-1)^nn}{n^2+15}}=\limm-\dfrac{n^3+n^2+15n+15}{n^3+2n^2+16n}=-1$
			\item $\dsum_{n=1}\dfrac{2^n\cos n}{n!}\\\limm\dfrac{a_{n+1}}{a_n}=\limm\dfrac{\dfrac{2^{n+1}\cos(n+1)}{(n+1)!}}{\dfrac{2^n\cos n}{n!}}=\limm\dfrac{2\cos(n+1)}{(n+1)\cos n}=0\Rightarrow$ ряд збіжний
 
		\end{enumerate}
	\end{enumerate}
\end{document}