\documentclass[a4paper,12pt]{article}

\usepackage[ukrainian,english]{babel}
\usepackage{ucs}
\usepackage[utf8]{inputenc}
\usepackage[T2A]{fontenc}

\usepackage{amsmath}
\usepackage{amsfonts}
\usepackage{amssymb}
\usepackage[document]{ragged2e}
\usepackage{graphicx}
\usepackage{wrapfig}
\usepackage{enumitem}
\usepackage{subfigure}

\usepackage{color,soul}
\setul{0.5ex}{0.3ex}

\usepackage[left=20mm, top=20mm, right=20mm, bottom=20mm, nohead, nofoot]{geometry}

\usepackage{tikz,pgfplots}
\usetikzlibrary{arrows.meta} 
\usetikzlibrary{shapes}

\makeatletter
\newcommand{\skipitems}[1]{%
  \addtocounter{\@enumctr}{#1}%
}
\makeatother

\newcommand\tab[1][0.5cm]{\hspace*{#1}}
\newcommand\dx[1]{\hspace*{0.2cm}\textrm{d}{#1}\hspace*{0.1cm}}
\newcommand\Res[1]{\hspace*{0.2cm}\underset{#1}{\textrm{Res}}\hspace*{0.1cm}}
\newcommand\dint[0]{\displaystyle\int}
\newcommand\doint[0]{\displaystyle\oint}
\newcommand{\Int}[0]{\mathfrak{I}}

\newcommand*\circled[1]{\tikz[baseline=(char.base)]{
            \node[shape=circle,draw,inner sep=2pt] (char) {#1};}}
 

\renewcommand{\Im}[0]{\mathfrak{Im}}
\renewcommand{\Re}[0]{\mathfrak{Re}}

\begin{document}
	\begin{justify}
		\thispagestyle{empty}\setlength{\parindent}{0pt}
  		\topskip0pt
 		\vspace*{\fill}
  		\begin{center}
  			\noindent\makebox[\linewidth]{\rule{\paperwidth}{0.4pt}}
   			\LARGE{\bigbreak ДОМАШНЯ РОБОТА №12\\З ПРЕДМЕТУ\\''ТЕОРІЯ ФУНКЦІЇ КОМПЛЕКСНОЇ ЗМІННОЇ''\\\bigbreak} 
   			ФІ-12 Бекешева Анастасія 
   			\noindent\makebox[\linewidth]{\rule{\paperwidth}{0.4pt}}
  		\end{center}
 		\vspace*{\fill}\newpage
 		\begin{enumerate}
 			\item \begin{enumerate}
 				\item $\dint\limits_0^{2\pi}\dfrac{\dx{t}}{\sqrt{21}\sin t+5}=\dint\limits_{|z|=1}\dfrac{\dx{z}}{iz\left(\sqrt{21}\dfrac1{2i}\left(z-\dfrac1z\right)+5\right)}=\left\langle\begin{array}{c}
 					\dfrac12\sqrt{21}z^2+5iz-\dfrac12\sqrt{21}=0 \\z=-i\sqrt{\dfrac37},z=-i\sqrt{\dfrac73}\\z=-i\sqrt{\dfrac37}\textrm{ полюс I порядку}
 				\end{array}\right\rangle=\\=\dint\limits_{|z|=1}\dfrac{\dx{z}}{\dfrac{\sqrt{21}}2\left(z+i\sqrt{\dfrac37}\right)\left(z+i\sqrt{\dfrac73}\right)}=2\pi i\Res{z=-i\sqrt{\frac37}}\dfrac{1}{\dfrac{\sqrt{21}}2\left(z+i\sqrt{\dfrac37}\right)\left(z+i\sqrt{\dfrac73}\right)}=\\=2\pi i\lim_{z\to-i\sqrt{\frac37}}\dfrac{1}{\dfrac{\sqrt{21}}2\left(z+i\sqrt{\dfrac73}\right)}=-\dfrac{i\sqrt{21}}{4}\cdot\dfrac2{\sqrt{21}}\cdot2\pi i =\pi$ 
 			\end{enumerate}
 			\item \begin{enumerate}
 				\item $\dint\limits_{-\infty}^{\infty}\dfrac{x^2+10}{(x^2+4)^2}\dx{x}=\dint\limits_{-\infty}^{\infty}\dfrac{(x-i\sqrt5)(x+i\sqrt5)}{(x-2i)^2(x+2i)^2}\dx{x}=2\pi i\Res{z=2i}\dfrac{z^2+10}{(z^2+4)^2}=\\=2\pi i\lim_{z\to2i}\dfrac{\dx{}}{\dx{z}}\left(\dfrac{z^2+10}{(z+2i)^2}\right)=2\pi i\lim_{z\to2i}\dfrac{2z(z+2i)^2-2(z^2+10)(z+2i)}{(z+2i)^3}=\\=2\pi i\lim_{z\to2i}\dfrac{4iz-20}{(z+2i)^3}=2\pi i\dfrac{-28}{-64i}=\dfrac78\pi, \langle 2i\textrm{ полюс II порядку}\rangle$
 				\item $\dint\limits_{-\infty}^{\infty}\dfrac{\dx{x}}{(x^2+1)^4}=2\pi i\Res{z\to i}\dfrac{1}{(z-i)^4(z+i)^4}=\dfrac13\pi i\lim_{z\to i}\dfrac{\dx{}^3}{\dx{z}^3}\left(\dfrac{1}{(z+i)^4}\right)=\\=\left\langle\dfrac{\dx{}^3}{\dx{z}^3}\left(\dfrac{1}{(z+i)^4}\right)= \dfrac{\dx{}^2}{\dx{z}^2}\left(-\dfrac{4}{(z+i)^5}\right)=\dfrac{\dx{}}{\dx{z}}\left(\dfrac{20}{(z+i)^6}\right)=-\dfrac{120}{(z+i)^7}\right\rangle=\\= \dfrac13\pi i\lim_{z\to i}\dfrac{-120}{(z+1)^7}=\pi\dfrac{120}{3\cdot 2^7}=\dfrac5{16}\pi,\langle i\textrm{ полюс IV порядку}\rangle$
 			\end{enumerate}
 			\item \begin{enumerate}
 				\item $\dint\limits_{0}^{\infty}\dfrac{\cos2x}{\left(x^2+\dfrac14\right)^2}\dx{x}=\dfrac12\dint\limits_{-\infty}^{\infty}\dfrac{\cos2x}{\left(x^2+\dfrac14\right)^2}\dx{x}=\dfrac12\Re\left[2\pi i\Res{z=\frac i2}\dfrac{e^{2iz}}{\left(z^2+\dfrac14\right)^2}\right]=\\=\dfrac12\Re\left[2\pi i\lim_{z\to\frac i2}\dfrac{\dx{}}{\dx{z}}\left(\dfrac{e^{2iz}}{\left(z+\dfrac i2\right)^2}\right)\right]=\dfrac12\Re\left[2\pi i\lim_{z\to\frac i2}\dfrac{e^{2iz}2i(z+\frac i2)^2-e^{2iz}(2z+i)}{\left(z+\dfrac i2\right)^4}\right]=\\=\dfrac12\Re\left[2\pi i\dfrac{e^{-1}2i^3-e^{-1}2i}{i^4}\right]=\dfrac12\Re\left[4\pi e^{-1}+4\pi e^{-1}\right]=\dfrac{4\pi}{e}$
 				\item $\dint\limits_{-\infty}^{\infty}\dfrac{(x^3+1)\sin x}{x^4+5x^2+4}\dx{x}=\Im\left[2\pi i\Res{z=2i}\dfrac{(z^3+1)e^{iz}}{(z^2+4)(z^2+1)}+2\pi i\Res{z=i}\dfrac{(z^3+1)e^{iz}}{(z^2+4)(z^2+1)}\right]=\\=\Im\left[2\pi i\dfrac{(z^3+1)e^{iz}}{4z^3+10z}\bigg|_{2i}+2\pi i\dfrac{(z^3+1)e^{iz}}{4z^3+10z}\bigg|_{i}\right]=\Im\left[\dfrac{2\pi i\cdot (-8i+1)\cdot e^{-2}}{-32i+20i}\right.+\\+\left.\dfrac{2\pi i\cdot(-i+1)\cdot e^{-1}}{-4i+10i}\right]=\Im\left[-\dfrac\pi{6e^2}+\dfrac{4\pi i}{3e^2}-\dfrac\pi{3e}-\dfrac{\pi i}{3e}\right]=\left(\dfrac{4\pi -\pi  e}{3e^2}\right)=\dfrac{\pi (4-e)}{3e^2}$
 			\end{enumerate}
 		\end{enumerate}
 	\end{justify}
\end{document}