\documentclass[a4paper,12pt]{article}

\usepackage[ukrainian,english]{babel}
\usepackage{ucs}
\usepackage[utf8]{inputenc}
\usepackage[T2A]{fontenc}

\usepackage{amsmath}
\usepackage{amsfonts}
\usepackage{amssymb}
\usepackage[document]{ragged2e}
\usepackage{graphicx}
\usepackage{wrapfig}
\usepackage{enumitem}
\usepackage{subfigure}

\usepackage{color,soul}
\setul{0.5ex}{0.3ex}

\usepackage[left=20mm, top=20mm, right=20mm, bottom=20mm, nohead, nofoot]{geometry}

\usepackage{tikz,pgfplots}
\usetikzlibrary {arrows.meta} 

\newcommand\tab[1][0.5cm]{\hspace*{#1}}
\newcommand\dx[1]{\hspace*{0.2cm}\textrm{d}{#1}\hspace*{0.1cm}}
\newcommand\dint[0]{\displaystyle\int}

\renewcommand{\Im}[0]{\mathfrak{Im}}
\renewcommand{\Re}[0]{\mathfrak{Re}}
\begin{document}
	\begin{justify}
		\thispagestyle{empty}\setlength{\parindent}{0pt}
  		\topskip0pt
 		\vspace*{\fill}
  		\begin{center}
  			\noindent\makebox[\linewidth]{\rule{\paperwidth}{0.4pt}}
   			\LARGE{\bigbreak ДОМАШНЯ РОБОТА №6\\З ПРЕДМЕТУ\\''ТЕОРІЯ ФУНКЦІЇ КОМПЛЕКСНОЇ ЗМІННОЇ''\\\bigbreak} 
   			ФІ-12 Бекешева Анастасія 
   			\noindent\makebox[\linewidth]{\rule{\paperwidth}{0.4pt}}
  		\end{center}
 		\vspace*{\fill}\newpage
 		\begin{enumerate}
 		\item 	
 		\begin{enumerate}
 			\item $z_1=0,\tab z_2=2-i$
 				$\\y=-\dfrac12x\Rightarrow z=-\dfrac12ix+x=x\left(1-\dfrac12i\right),\tab x:0\to2\\\dx{z}=\left(1-\dfrac12i\right)\dx{x},\tab |z|=\left|x\left(1-\dfrac12i\right)\right|=\dfrac{\sqrt5}2|x|\\\dint\limits_C|z|\dx{z}=\dint\limits_0^2\dfrac{\sqrt5}2\left(1-\dfrac12i\right)|x|\dx{x}=\dfrac{\sqrt5}2\left(1-\dfrac12i\right)\dfrac{x^2}{2}\bigg|_{0}^2=\sqrt5\left(1-\dfrac12i\right)$
 			\item $z_1=-i,\tab z_2=i$
 				$\\x=0,\tab y:-1\to1\Rightarrow z=iy\\\dx{z}=i\dx{y},\tab|z|=|y|\\\dint\limits_C|z|\dx{z}=i\dint\limits_{-1}^1|y|\dx{y}=2i\dint\limits_0^1 y\dx{y}=2i\cdot\dfrac{y^2}{2}\bigg|_0^1=i$
			\item $|z|=1,\tab -\dfrac\pi2\leq\arg z\leq\dfrac\pi2$
				$z=z_0+R\cdot e^{i\varphi}=0+1\cdot e^{i\varphi}=e^{i\varphi}\\\varphi:-\dfrac\pi2\to\dfrac\pi2,\tab \dx{z}=ie^{i\varphi}\dx{\varphi}\\\dint\limits_C|z|\dx{z}=\dint\limits_{-\frac{\pi}{2}}^{\frac{\pi}{2}}ie^{i\varphi}\dx{\varphi}=e^{i\varphi}\bigg|_{-\frac{\pi}{2}}^{\frac{\pi}{2}}=e^{i\frac\pi2}-e^{-i\frac\pi2}=\cos\dfrac{\pi}{2}+i\sin\dfrac{\pi}{2}-\cos-\dfrac{\pi}{2}-\\-i\sin-\dfrac{\pi}{2}=0+i-0+i=2i$
 				\begin{figure*}[htp]\centering
 					\begin{tikzpicture}[scale=0.6]
 						\begin{axis}[ticks=none,axis lines=middle, xmin=-0.5, xmax=0.5,ymin=-0.5,ymax=0.5]	
						\end{axis}
						\draw (3.43,2.85) node[circle,fill,inner sep=1pt] {};
						\draw (5,2) node[circle,fill,inner sep=1pt] {};
						\draw[->] (3.43,2.85) node[below] {$z_1$} -- (5,2) node[right] {$z_2$};
						\draw (3.43, -0.5) node {(a)};
 					\end{tikzpicture}\tab 
 					\begin{tikzpicture}[scale=0.6]
 						\begin{axis}[ticks=none,axis lines=middle, xmin=-0.5, xmax=0.5,ymin=-0.5,ymax=0.5]	
						\end{axis}
						\draw (3.43,1.85) node[circle,fill,inner sep=1pt] {};
						\draw (3.43,3.85) node[circle,fill,inner sep=1pt] {};
						\draw[->] (3.43,1.85) node[left] {$z_1$} -- (3.43,3.85) node[right] {$z_2$};
						\draw (3.43, -0.5) node {(b)};
 					\end{tikzpicture}\tab 
 					\begin{tikzpicture}[scale=0.6]
 						\begin{axis}[ticks=none,axis lines=middle, xmin=-0.5, xmax=0.5,ymin=-0.5,ymax=0.5]	
						\end{axis}
						\draw (3.43,1.85) node[left] {$z_1$} node[circle,fill,inner sep=1pt] {};
						\draw (3.43,3.85) node[left] {$z_2$} node[circle,fill,inner sep=1pt] {};
						\draw[->] (3.43,1.85) arc (-90:90:1);
						\draw (3.43, -0.5) node {(c)};
 					\end{tikzpicture}

 				\end{figure*}\\
 		\end{enumerate}
 		\item \begin{enumerate}
 			\item $z_1=0,\tab z_2=1+i\\y=x,\tab x:0\to1,\tab z=x+ix=x(i+1),\tab \dx{z}=(1+i)\dx{x}\\\dint\limits_C(x-y+ix^2)\dx{z}=\dint\limits_0^1(x-x+ix^2)\cdot(1+i)\dx{x}=\dint\limits_0^1x^2(i-1)\dx{x}=\\=(i-1)\dfrac{x^3}3\bigg|_0^1=\dfrac13(i-1)$
 			\item $y=0:\tab x:0\to1,\tab z=x,\tab \dx{z}=\dx{x},\\x=1:\tab y:0\to 1,\tab z=1+iy,\tab \dx{z}=i\dx{y},\\\dint\limits_C(x-y+ix^2)\dx{z}=\dint\limits_0^1(x+ix^2)\dx{x}+\dint\limits_0^1(1-y+i)i\dx{y}=\dfrac{x^2}2\bigg|_0^1+i\dfrac{x^3}3\bigg|_0^1-\dfrac{iy^2}2\bigg|_0^1+\\+(1+i)iy\bigg|_0^1=\dfrac12+i\dfrac13+i-\dfrac i2-1=1+i\left(\dfrac13+1-\dfrac12\right)=-\dfrac12+i\dfrac56$
 			\item $x=0:\tab y:0\to1,\tab z=iy,\tab \dx{z}=i\dx{y},\\y=1:\tab x:0\to1,\tab z=x+i,\tab \dx{z}=\dx{x},\\\dint\limits_C(x-y+ix^2)\dx{z}=\dint\limits_0^1(-iy)\dx{y}+\dint\limits_0^1(x-1+ix^2)\dx{x}=-i\dfrac{y^2}2\bigg|_0^1+\dfrac{x^2}2\bigg|_0^1-x\bigg|_0^1+\\-\dfrac12-\dfrac i6$
 			
 			\begin{figure*}[htp]\centering
 				\begin{tikzpicture}[scale=0.6]
 					\begin{axis}[ticks=none,axis lines=middle, xmin=-0.5, xmax=0.5,ymin=-0.5,ymax=0.5]	
					\end{axis}
					\draw (3.43,2.85) node[circle,fill,inner sep=1pt] {};
					\draw (4.45,4) node[circle,fill,inner sep=1pt] {};
					\draw[->] (3.43,2.85) node[below] {$z_1$} -- (4.45,4) node[right] {$z_2$};
					\draw (3.43, -0.5) node {(a)};
 				\end{tikzpicture}\tab 
 				\begin{tikzpicture}[scale=0.6]
 					\begin{axis}[ticks=none,axis lines=middle, xmin=-0.5, xmax=0.5,ymin=-0.5,ymax=0.5]	
					\end{axis}
					\draw (3.43,2.85) node[circle,fill,inner sep=1pt] {};
					\draw (4.45,4) node[circle,fill,inner sep=1pt] {};
					\draw (4.45,2.85) node[circle,fill,inner sep=1pt] {};
					\draw[->] (3.43,2.85) node[below] {$z_1$} -- (4.45,2.85) -- (4.45,4) node[right] {$z_2$};
					\draw (3.43, -0.5) node {(b)};
 				\end{tikzpicture}\tab 
 				\begin{tikzpicture}[scale=0.6]
 					\begin{axis}[ticks=none,axis lines=middle, xmin=-0.5, xmax=0.5,ymin=-0.5,ymax=0.5]	
					\end{axis}
					\draw (3.43,2.85) node[circle,fill,inner sep=1pt] {};
					\draw (4.45,4) node[circle,fill,inner sep=1pt] {};
					\draw (3.43,4) node[circle,fill,inner sep=1pt] {};
					\draw[->] (3.43,2.85) node[below] {$z_1$} -- (3.43,4) -- (4.45,4) node[right] {$z_2$};
					\draw (3.43, -0.5) node {(c)};
 				\end{tikzpicture}
 			\end{figure*}

 		\end{enumerate}
 		\item \begin{enumerate} 
 			\item $z_1,=-2,\tab z_2=2,\\z=2e^{i\varphi},\tab\varphi:\pi\to2\pi,\tab\dx{z}=2ie^{i\varphi}\dx{\varphi},\tab |z|=2,\\\dint\limits_Lz|z|\dx{z}=\dint\limits_\pi^{2\pi}2\cdot 2e^{i\varphi}\cdot 2ie^{i\varphi}\dx{\varphi}=8i\dint\limits_\pi^{2\pi}e^{2i\varphi}\dx{\varphi}=-\dfrac i2\cdot 8i\dint\limits_\pi^{2\pi}e^{2i\varphi}\dx{(2i\varphi)}=\\=4e^{2i\varphi}\Big|_\pi^{2\pi}=4(e^{4\pi i}-e^{2\pi i})=4e^{2\pi i}(e^{2\pi i}-1)=4\cdot(\cos2\pi+i\sin2\pi)\cdot(\cos2\pi+i\sin2\pi-1)\\=4\cdot(1+i\cdot0)\cdot(1+i\cdot 0-1)=4\cdot1\cdot0=0$
 			\addtocounter{enumii}{1}
 			\item $z_1=0,\tab z_2=\dfrac12+i\dfrac{\sqrt3}2,\\y=\sqrt3x,\tab x:0\to\dfrac12,\tab z=x+i\sqrt3 x,\tab \dx{z}=(1+i\sqrt3)\dx{x},\\\dint\limits_Le^{|z|^2}\Re z\dx{z}=\dint\limits_0^{\frac12}x(1+i\sqrt3)e^{\sqrt{x^2+3x^2}^2}\dx{x}=(1+i\sqrt3)\dint\limits_0^{\frac12}e^{4x^2}\dx{x}=\dfrac{(1+i\sqrt3)}2\cdot\\\cdot\dint\limits_0^{\frac12}\dfrac1xe^{x^2}\dx{(4x^2)}=\dfrac{(1+i\sqrt3)}2\cdot\dfrac{e^{4x^2}}4\Bigg|_0^{\frac12}=\dfrac{(1+i\sqrt3)}8(e-1)$
 			\item $|z-1|=1,\tab z=e^{i\varphi},\tab \varphi:0\to2\pi,\tab \dx{z}=ie^{i\varphi}\dx{\varphi},\\\Re(z)=\Re(e^{i\varphi})=\Re(\cos\varphi+i\sin\varphi)=\cos\varphi\\\displaystyle\oint\limits_{|z-1|=1}\Re(z)\dx{z}=\dint\limits_0^{2\pi}\cos\varphi\cdot ie^{i\varphi}\dx{\varphi}=-i\cdot i\dint\limits_0^{2\pi}e^{i\varphi}\ch i\varphi\dx{(i\varphi)}=\dint\limits_0^{2\pi}\dfrac14\cdot 2e^{2i\varphi}\cdot \\\cdot e^{-2i\varphi}(e^{2i\varphi}+1)\dx{(i\varphi)}=\left\langle t= e^{2i\varphi},\tab \dx{(i\varphi)}=\dfrac12 e^{-2i\varphi}\dx{t}\right\rangle=\dfrac14\dint\limits_0^{2\pi}\dfrac{t+1}t\dx{t}=\\=\dfrac14\dint\limits_0^{2\pi}\left(\dfrac1t+1\right)\dx{t}=\dfrac14\ln t+\dfrac14 t\Bigg|_0^{2\pi}=\dfrac12 i\varphi+\dfrac14 e^{2i\varphi}\Bigg|_0^{2\pi}=i\pi+\dfrac14 e^{4i\pi}-0-\dfrac14e^0=\\=i\pi-\dfrac14+\dfrac14(\cos 4\pi +i\sin4\pi)=i\pi-\dfrac14+\dfrac14=i\pi$
 			
 			\begin{figure*}[htp]\centering
 				\begin{tikzpicture}[scale=0.6]
 					\begin{axis}[ticks=none,axis lines=middle, xmin=-0.5, xmax=0.5,ymin=-0.5,ymax=0.5]	
					\end{axis}
					\draw (2.43,2.85) node[above] {$z_1$} node[circle,fill,inner sep=1pt] {};
					\draw (4.43,2.85) node[above] {$z_2$} node[circle,fill,inner sep=1pt] {};
					\draw[->] (2.43,2.85) arc (-180:0:1);
					\draw (3.43, -0.5) node {(a)};
 				\end{tikzpicture}\tab 
 				\begin{tikzpicture}[scale=0.6]
 					\begin{axis}[ticks=none,axis lines=middle, xmin=-0.5, xmax=0.5,ymin=-0.5,ymax=0.5]	
					\end{axis}
					\draw (3.43,2.85) node[circle,fill,inner sep=1pt] {};
					\draw (4,4) node[circle,fill,inner sep=1pt] {};
					\draw[->] (3.43,2.85) node[below] {$z_1$} -- (4,4) node[right] {$z_2$};
					\draw (3.43, -0.5) node {(c)};
 				\end{tikzpicture}\tab  
 				\begin{tikzpicture}[scale=0.6]
 					\begin{axis}[ticks=none,axis lines=middle, xmin=-0.5, xmax=0.5,ymin=-0.5,ymax=0.5]	
					\end{axis}
					\draw (4.43,2.85) node[above] {$1$} node[circle,fill,inner sep=1pt] {};
					\draw[->] (5.43,2.85) arc (0:360:1);
					\draw (3.43, -0.5) node {(a)};
 				\end{tikzpicture}
 			\end{figure*}$\\\\\\\\$
 		\end{enumerate}
 			
 		\end{enumerate}
 	\end{justify}
\end{document}