\documentclass[a4paper,12pt]{article}

\usepackage[ukrainian,english]{babel}
\usepackage{ucs}
\usepackage[utf8]{inputenc}
\usepackage[T2A]{fontenc}

\usepackage{amsmath}
\usepackage{amsfonts}
\usepackage{amssymb}
\usepackage[document]{ragged2e}
\usepackage{graphicx}
\usepackage{wrapfig}
\usepackage{enumitem}
\usepackage{subfigure}

\usepackage{color,soul}
\setul{0.5ex}{0.3ex}

\usepackage[left=20mm, top=20mm, right=20mm, bottom=20mm, nohead, nofoot]{geometry}

\usepackage{tikz,pgfplots}
\usetikzlibrary {arrows.meta} 

\makeatletter
\newcommand{\skipitems}[1]{%
  \addtocounter{\@enumctr}{#1}%
}
\makeatother

\newcommand\tab[1][0.5cm]{\hspace*{#1}}
\newcommand\dx[1]{\hspace*{0.2cm}\textrm{d}{#1}\hspace*{0.1cm}}
\newcommand\dint[0]{\displaystyle\int}

\renewcommand{\Im}[0]{\mathfrak{Im}}
\renewcommand{\Re}[0]{\mathfrak{Re}}
\begin{document}
	\begin{justify}
		\thispagestyle{empty}\setlength{\parindent}{0pt}
  		\topskip0pt
 		\vspace*{\fill}
  		\begin{center}
  			\noindent\makebox[\linewidth]{\rule{\paperwidth}{0.4pt}}
   			\LARGE{\bigbreak ДОМАШНЯ РОБОТА №8\\З ПРЕДМЕТУ\\''ТЕОРІЯ ФУНКЦІЇ КОМПЛЕКСНОЇ ЗМІННОЇ''\\\bigbreak} 
   			ФІ-12 Бекешева Анастасія 
   			\noindent\makebox[\linewidth]{\rule{\paperwidth}{0.4pt}}
  		\end{center}
 		\vspace*{\fill}\newpage
 		\begin{enumerate}
 			\item $\dfrac{1}{z+1}=\dfrac{1}{1-(-z)}=\sum\limits_{n=0}^\infty(-z)^n=\sum\limits_{n=0}^\infty(-1)(z)^n,\tab |z|<1\\$
 				\begin{figure*}[htp]\centering
 					\begin{tikzpicture}
 						\begin{axis}[ticks=none,axis lines=middle, xmin=-0.5, xmax=0.5,ymin=-0.5,ymax=0.5 ]	
						\end{axis}
						\draw (5.43,2.85) node[anchor = south west] {$1$}  node[circle,fill,inner sep=1pt,color=red] {};
						\draw (3.43,2.85) circle (2);
						\draw (3.43, -0.5) node {(a)};
 					\end{tikzpicture}
 				\end{figure*}
 			\skipitems{1}
 			\item \begin{enumerate} 
 				\skipitems{2} 
 				\item $f(z)=(z-3)\cos\pi\dfrac{z-3}{z}=(z-3)\cos\left(\pi-\dfrac{3\pi}{z}\right)=-(z-3)\cos\left(\dfrac{3\pi}{z}\right)=\\=-(z-3)\sum\limits_{n=0}^\infty\dfrac{(-1)^n\left(\dfrac{3\pi}z\right)^{2n}}{(2n)!}=\sum\limits_{n=0}^\infty\dfrac{(-1)^{n+1}3^{2n}\pi^{2n}}{(2n)!z^{2n-1}}+\sum\limits_{n=0}^\infty\dfrac{(-1)^{n}3^{2n+1}\pi^{2n}}{(2n)!z^{2n}}$
 			\end{enumerate}
 		\end{enumerate}
 	\end{justify}
\end{document}