\documentclass[a4paper,12pt]{article}
\usepackage[ukrainian,english]{babel}
\usepackage{ucs}
\usepackage[utf8]{inputenc}
\usepackage[T2A]{fontenc}
\usepackage{amsmath}
\usepackage{fleqn}
\usepackage{amsfonts}
\usepackage{enumerate}
\usepackage{multicol}
\usepackage{forest}
\usepackage{graphicx}
\usetikzlibrary{arrows.meta}
\tikzset{
  0 my edge/.style={densely dashed, my edge},
  my edge/.style={-{Stealth[]}},
}
\forestset{
  BDT/.style={
    for tree={
      if n children=0{}{circle},% use a circle unless there are 0 children
      draw,% draw every node
      edge={
        my edge,% use the my edge style for edges (with the arrow)
      },
      if n=1{
        edge+={0 my edge},% if the child is the first one, add the 0 my edge style (dashed)
      }{},
      font=\rmfamily,% use sans serif for node text
    }
  },
}
\DeclareMathOperator{\cnf}{cnf}
\newcommand\tab[1][1cm]{\hspace*{#1}}
\usepackage[left=20mm, top=20mm, right=10mm, bottom=20mm, nohead, nofoot]{geometry}
\begin{document}
\begin{titlepage}
    \begin{center}
        \vspace*{1cm}
            
        \Huge
        \textbf{Домашня контрольна робота}
            
        \vspace{0.5cm}
        \LARGE
        Варіант №12002
            
        \vspace{1.5cm}
            
        \textbf{Бекешева Анастасія}
            
        \vfill
            
        Part I
            
        \vspace{0.8cm}
            

            
        \Large
        ФІ-12\\01.06.2022
            
    \end{center}
\end{titlepage}
\begin{enumerate}
	\item $\left(L_1^RL_2^R\right)^+=\left(\left(L_1^R \right)^+\cup \left(L_2^R \right)^*\right)^+\\$ \begin{align*}
		L_1^R&=\left\{x\in\Sigma^*\>|\>x^R\in L_1\right\}\\
		L_2^R&=\left\{y\in\Sigma^*\>|\>y^R\in L_1\right\}\\
		L_1^RL_2^R&=\left\{xy\in\Sigma^*\>|\>x^R\in L_1,\>y^R\in L_2^R\right\}\\
		\left(L_1^RL_2^R\right)^+&=\left\{xy\in\Sigma^*\>|\>\exists n\in\mathbb{N}_1,\>x^R\in L_1^n,\>y^R\in L_2^n\right\}
	\end{align*}
	\begin{align*}
		L_1^R&=\left\{x\in\Sigma^*\>|\>x^R\in L_1\right\}\\
		L_2^R&=\left\{y\in\Sigma^*\>|\>y^R\in L_1\right\}\\
		\left(L_1^R\right)^+&=\left\{x\in\Sigma^*\>|\>\exists n\in\mathbb{N}_1,\>x^R\in L_1^n\right\}\\
		\left(L_2^R\right)^*&=\left\{x\in\Sigma^*\>|\>\exists n\in\mathbb{N}_0,\>x^R\in L_2^n\right\}\\
		\left(L_1^R \right)^+\cup \left(L_2^R \right)^*&=\{z\in\Sigma^*\>|\>\exists n\in\mathbb{N}_1,\>z^R\in L_1^n\lor z^R\in L_2^n\}\\
		\left(\left(L_1^R \right)^+\cup \left(L_2^R \right)^*\right)^+&=\{z\in\Sigma^*\>|\>\exists n\in\mathbb{N}_1,\>\>z^R\in L_1^n\lor z^R\in L_2^n \}
	\end{align*}\\$\Rightarrow\left(L_1^RL_2^R\right)^+\neq\left(\left(L_1^R \right)^+\cup \left(L_2^R \right)^*\right)^+$ \\Let $\Sigma=\{\alpha_1,\>\alpha_2,\>\beta_1,\>\beta_2\},\>L_1=\{\alpha_1,\>\alpha_1\alpha_2\},\>L_2=\{\beta_1,\>\beta_1\beta_2\}.$
	\begin{align*}
		L_1^R&=\left\{\alpha_1,\>\alpha_2\alpha_1\right\}\\
		L_2^R&=\left\{\beta_1,\>\beta_2\beta_1\right\}\\
		L_1^RL_2^R&=\left\{\alpha_1\beta_1,\>\alpha_1\beta_2\beta_1,\>\alpha_2\alpha_1\beta_1,\>\alpha_2\alpha_2\beta_2\beta_2\right\}\\
		\left(L_1^RL_2^R\right)^+&=\left\{\alpha_1\beta_1\alpha_1\beta_1,\>\alpha_1\beta_2\beta_1\alpha_1\beta_2\beta_1,\>\alpha_2\alpha_1\beta_1\alpha_2\alpha_1\beta_1\dots \right\}
	\end{align*}
	\begin{align*}
		L_1^R&=\left\{\alpha_1,\>\alpha_2\alpha_1\right\}\\
		L_2^R&=\left\{\beta_1,\>\beta_2\beta_1\right\}\\
		\left(L_1^R\right)^+&=\left\{\alpha_1,\>\alpha_2\alpha_1,\>\alpha_1\alpha_1,\>\alpha_2\alpha_1\alpha_2\alpha_1\dots\right\}\\
		\left(L_2^R\right)^*&=\left\{\varepsilon,\>\beta_1,\>\beta_2\beta_1,\>\beta_1\beta_1,\>\beta_2\beta_1\beta_2\beta_1\dots\right\}\\
		\left(L_1^R \right)^+\cup \left(L_2^R \right)^*&=\{\varepsilon,\>\alpha_1,\>\alpha_2\alpha_1,\>\alpha_1\alpha_1,\>\alpha_2\alpha_1\alpha_2\alpha_1,\>\beta_1,\>\beta_2\beta_1,\>\beta_1\beta_1,\>\beta_2\beta_1\beta_2\beta_1\dots \}\\
		\left(\left(L_1^R \right)^+\cup \left(L_2^R \right)^*\right)^+&=\{\alpha_1,\>\alpha_2\alpha_1,\>\alpha_1\alpha_1,\alpha_1\alpha_1\alpha_1\>\>\alpha_2\alpha_1\alpha_2\alpha_1,\>\beta_1,\>\beta_2\beta_1,\>\beta_1\beta_1,\>\beta_1\beta_1\beta_1\>\beta_2\beta_1\beta_2\beta_1\dots \}
	\end{align*}
	\item $A=P\land R\to\neg(Q\leftrightarrow\neg P\land R)$
		\begin{align*}
			\cnf(A)&=\neg(P\land R)\lor\neg(Q\leftrightarrow\neg P\land R)=\\&=\neg(P\land R)\lor\neg((Q\lor\neg(\neg P\land R))\land(\neg Q\lor(\neg P\land R)))=\\&=\neg P\lor\neg R\lor((\neg Q\land\neg P\land R)\lor (Q\land(P\lor\neg R)))=\\&=(\neg P\lor \neg R\lor Q)\land (\neg P\lor \neg R\lor P\lor\neg R)\lor (\neg Q\land\neg P\land R)=\\&=(\neg P\lor \neg R\lor Q)\lor (\neg Q\land\neg P\land R)=\\&=((\neg P\lor \neg R\lor Q)\lor\neg Q)\land((\neg P\lor \neg R\lor Q)\lor(\neg P\lor R))=\\&=\neg P\lor\neg R\lor Q
		\end{align*}
		\\\\\emph{\textbf{Tseitin:}}\\
		\begin{align*}
			\mathcal{T}(a)\backslash\mathcal{T}_0(A)&=\{(\neg P),(P\land R),(\neg P\land R),(Q\leftrightarrow\neg P\land R),\\&(\neg(Q\leftrightarrow\neg P\land R)),(P\land R\to\neg(Q\leftrightarrow\neg P\land R))\}
		\end{align*}t
		\begin{align*}
			\textrm{substitute } \neg P\textrm{ with }S_1&&\\P\land R\textrm{ with }S_2&&\\
			\tilde{\varphi_T}(A)&=1\land(S_1\leftrightarrow\neg P)\land(S_2\leftrightarrow P\land R)&\\A_1&=S_2\to\neg(Q\leftrightarrow S_1\land R)&\\\textrm{substitute } S_1\land R\textrm{ with }S_3&&\\\tilde{\varphi_T}(A)&=1\land(S_1\leftrightarrow\neg P)\land(S_2\leftrightarrow P\land R)\land(S_3\leftrightarrow S_1\land R)&\\A_2&=S_2\to\neg(Q\leftrightarrow S_3)&\\\textrm{substitute } Q\leftrightarrow S_3\textrm{ with }S_4&&\\\tilde{\varphi_T}(A)&=1\land(S_1\leftrightarrow\neg P)\land(S_2\leftrightarrow P\land R)\land(S_3\leftrightarrow S_1\land R)\land&\\&\land(S_4\leftrightarrow(Q\leftrightarrow S_3))&\\A_3&=S_2\to\neg(S_4)&\\\textrm{substitute } \neg S_4\textrm{ with }S_5&&\\\tilde{\varphi_T}(A)&=1\land(S_1\leftrightarrow\neg P)\land(S_2\leftrightarrow P\land R)\land(S_3\leftrightarrow S_1\land R)\land&\\&\land(S_4\leftrightarrow(Q\leftrightarrow S_3))\land(S_5\leftrightarrow \neg S_4) &\\A_4&=S_2\to S_5&\\\textrm{substitute } S_2\to S_5\textrm{ with }S_6\\\tilde{\varphi_T}(A)&=1\land(S_1\leftrightarrow\neg P)\land(S_2\leftrightarrow P\land R)\land(S_3\leftrightarrow S_1\land R)\land&\\&\land(S_4\leftrightarrow(Q\leftrightarrow S_3))\land(S_5\leftrightarrow \neg S_4)\land(S_6\leftrightarrow (S_2\to S_5))\land S_6 &\\ A_5&=S_6&
		\end{align*}
		\begin{align*}
			\cnf(\tilde{\varphi_T}(A))=& (P \lor S_1) \land (\neg S_1 \lor \neg P) \land (\neg P \lor \neg R \lor S_2) \land\\&\land (\neg S_2 \lor P) \land (\neg S_2 \lor R) \land (\neg S_1 \lor \neg R \lor S_3) \land (\neg S_3 \lor S_1) \land\\&\land (\neg S_3 \lor R) \land (\neg Q \lor \neg S_3 \lor S_4) \land (Q \lor S_3 \lor S_4) \land (\neg S_3 \lor Q \lor \neg S_4) \land\\&\land (\neg Q \lor S_3 \lor \neg S_4) \land (S_4 \lor S_5) \land (\neg S_5 \lor \neg S_4) \land (\neg S_2 \lor S_5) \land S_6=\\&=(\neg P\lor\neg R\lor S_2)\land(\neg P\lor \neg S_1)\land(P\lor\neg Q\lor\neg R\lor\neg S_5)\land\\&\land (P\lor S_1)\land(\neg Q\lor S_3\lor\neg S_4)\land (Q\lor\neg R\lor\neg S_4)\land(Q\lor S_3\lor\neg S_5)\land\\&\land(R\lor\neg S_2)\land(R\lor\neg S_3)\land(\neg S_2\lor\neg S_3)\land(S_4\lor S_5)\land S_6  
		\end{align*}
		Rank = $\left|\{P,Q,R,S_1,S_2,S_3,S_4,S_5,S_6\}\right|=9,$ Complexity = $\displaystyle\sum_{\land\in\cnf(\tilde{\varphi_T}(A)}1=11$ 
	\item $W = \{P_2 \lor P_4 \lor  \neg P_5, P_1 \lor  \neg P_2 \lor  \neg P_4, \neg P_1 \lor  \neg P_3 \lor P_5, P_1 \lor P_3 \lor  \neg P_4, \neg P_1 \lor  \neg P_4 \lor P_5, \neg P_2 \lor  \neg P_5 \lor  \neg P_2,
\neg P_1 \lor  P_3, P_2 \lor  \neg P_4, \neg P_2 \lor P_5\} \\\\\emph{\textbf{DPLL}:}\\$
	\begin{itemize}
		\item [\textbf{MULT}] $(\neg P_2 \lor  \neg P_5 \lor  \neg P_2)$\\$W_1 = \{P_2 \lor P_4 \lor  \neg P_5, P_1 \lor  \neg P_2 \lor  \neg P_4, \neg P_1 \lor  \neg P_3 \lor P_5, P_1 \lor P_3 \lor  \neg P_4, \neg P_1 \lor  \neg P_4 \lor P_5,\neg P_5\lor P_2, \neg P_1 \lor  P_3, P_2 \lor  \neg P_4, \neg P_2 \lor P_5\} $
		\item [\textbf{SUS}] $(\neg P_5\lor P_2)\\W_1 = \{P_1 \lor  \neg P_2 \lor  \neg P_4, \neg P_1 \lor  \neg P_3 \lor P_5, P_1 \lor P_3 \lor  \neg P_4, \neg P_1 \lor  \neg P_4 \lor P_5,\neg P_5\lor P_2, \neg P_1 \lor  P_3, P_2 \lor  \neg P_4, \neg P_2 \lor P_5\} $
		\item [\textbf{SPLIT}] $(P_1)\\W_{31} = \{\neg P_2 \lor  \neg P_4, P_3 \lor  \neg P_4, \neg P_5\lor P_2, P_2 \lor  \neg P_4, \neg P_2 \lor P_5\}\\W_{32} = \{\neg P_3 \lor P_5, \neg P_4 \lor P_5,\neg P_5\lor P_2, P_3, P_2 \lor  \neg P_4, \neg P_2 \lor P_5\}$
		\item [\textbf{UNIT}] $(P_3\in W_{32})\\W_{41} = \{\neg P_2 \lor  \neg P_4, P_3 \lor  \neg P_4, \neg P_5\lor P_2, P_2 \lor  \neg P_4, \neg P_2 \lor P_5\}\\W_{42} = \{P_5, \neg P_4 \lor P_5,\neg P_5\lor P_2,  P_2 \lor  \neg P_4, \neg P_2 \lor P_5\}$
		\item [\textbf{UNIT}] $(P_5\in W_{42})\\W_{41} = \{\neg P_2 \lor  \neg P_4, P_3 \lor  \neg P_4, \neg P_5\lor P_2, P_2 \lor  \neg P_4, \neg P_2 \lor P_5\}\\W_{42} = \{ \neg P_4 , P_2,  P_2 \lor  \neg P_4, \neg P_2 \}$
		\item [\textbf{UNIT}] $(P_2\in W_{42})\\W_{51} = \{\neg P_2 \lor  \neg P_4, P_3 \lor  \neg P_4, \neg P_5\lor P_2, P_2 \lor  \neg P_4, \neg P_2 \lor P_5\}\\W_{52} = \{ \neg P_4 , \neg P_4\}$
		\item [\textbf{SAME}] $(\neg P_4\in W_{52})\\W_{61} = \{\neg P_2 \lor  \neg P_4, P_3 \lor  \neg P_4, \neg P_5\lor P_2, P_2 \lor  \neg P_4, \neg P_2 \lor P_5\}\\W_{62} = \{ \neg P_4\}$
		\item [\textbf{UNIT}] $(\neg P_4\in W_{62})\\W_{71} = \{\neg P_2 \lor  \neg P_4, P_3 \lor  \neg P_4, \neg P_5\lor P_2, P_2 \lor  \neg P_4, \neg P_2 \lor P_5\}\\W_{72} = \O $
		\item [\textbf{PURE}] $(P_3\in W_{71})\\W_{81} = \{\neg P_2 \lor  \neg P_4,\neg P_4, \neg P_5\lor P_2, P_2 \lor  \neg P_4, \neg P_2 \lor P_5\}\\W_{72} = \O $
		\item [\textbf{UNIT}] $(\neg P_4\in W_{81})\\W_{91} = \{\neg P_2 , \neg P_5\lor P_2, P_2,  \neg P_2 \lor P_5\}\\W_{72} = \O $
		\item [\textbf{UNIT}] $( P_2\in W_{91})\\W_{101} = \{\neg P_5,P_5\}\\W_{72} = \O $
		\item [\textbf{UNIT}] $( P_5\in W_{101})\\W_{111} = \O\\W_{72} = \O $
	\end{itemize}W - unsatisfiable
	\\\\\emph{\textbf{Resolution}:}\\
	\begin{multicols}{3}
		\begin{enumerate}[(1)] 
			\item $P_2 \lor P_4 \lor  \neg P_5$
			\item $P_1 \lor  \neg P_2 \lor  \neg P_4$
			\item $\neg P_1 \lor  \neg P_3 \lor P_5$
			\item $ P_1 \lor P_3 \lor  \neg P_4$
			\item $\neg P_1 \lor  \neg P_4 \lor P_5$
			\item $\neg P_2 \lor  \neg P_5 \lor  \neg P_2$
			\item $\neg P_1 \lor  P_3$
			\item $P_2 \lor  \neg P_4$
			\item $\neg P_2 \lor P_5$
		\end{enumerate}
	\end{multicols}
	\begin{multicols}{2}
		\begin{enumerate}
			\item \begin{align*}
				P_2\lor\neg P_5\tab (1,8,P_4)
			\end{align*}
			\item \begin{align*}
				P_3\lor P_4\tab & (4,7,P_1)
			\end{align*}
			\item \begin{align*}
				P_2\lor P_3\tab (8,b,P_4)
			\end{align*}
			\item \begin{align*}
				\neg P_2\tab & (6,9,P_5) 
			\end{align*}
			\item \begin{align*}
				\neg P_5\tab & (a,d,P_2)
			\end{align*}
			\item \begin{align*}
				P_3\tab & (c,d,P_3)
			\end{align*}
			\item \begin{align*}
				\neg P_4\tab & (8,d,P_2)
			\end{align*}
			\item \begin{align*}
				\neg P_1\lor P_5\tab & (3,f,P_3)
			\end{align*}
			\item \begin{align*}
				\neg P_1\tab & (e,h,P_5)
			\end{align*}
		\end{enumerate}
	\end{multicols}
	\emph{\textbf{Resolution}:}\\
	\begin{multicols}{3}
		\begin{enumerate}[(1)] 
			\item $P_2 \lor P_4 \lor  \neg P_5$
			\item $P_1 \lor  \neg P_2 \lor  \neg P_4$
			\item $\neg P_1 \lor  \neg P_3 \lor P_5$
			\item $ P_1 \lor P_3 \lor  \neg P_4$
			\item $\neg P_1 \lor  \neg P_4 \lor P_5$
			\item $\neg P_2 \lor  \neg P_5 \lor  \neg P_2$
			\item $\neg P_1 \lor  P_3$
			\item $P_2 \lor  \neg P_4$
			\item $\neg P_2 \lor P_5$
		\end{enumerate}
	\end{multicols}
	\begin{multicols}{2}
		\begin{enumerate}
			\item \begin{align*}
				\neg P_4\lor\neg P_2\tab & (8,9,P_2)
			\end{align*}
			\item \begin{align*}
				P_1\lor\neg P_2\lor P_3\tab & (4,a,P_4)
			\end{align*}
			\item \begin{align*}
				P_1\lor P_4\lor P_3\lor\neg P_5\tab & (1,b,P_2) 
			\end{align*}		 
			\item \begin{align*}
				P_4\lor P_3\lor\neg P_5\tab (7,c,P_1)
			\end{align*}
			\item \begin{align*}
				\neg P_2 \lor P_3\lor P_4\tab & (9, d, P_5)
			\end{align*}
			\item \begin{align*}
				\neg P_1\lor\neg P_2\lor P_3\lor P_5\tab & (5,e,P_4)
			\end{align*}
			\item \begin{align*}
				\neg P_2\lor P_3\lor\neg P_4\lor P_5\tab & (2,e,P_1)
			\end{align*}
			\item \begin{align*}
				\neg P_1\lor\neg P_2\lor \neg P_4\lor P_5\tab & (3,h,P_3)
			\end{align*}
			\item \begin{align*}
				\neg P_1\lor\neg P_4\lor P_5\tab & (9,h,P_2)
			\end{align*}
			\item \begin{align*}
				\neg P_1\lor\neg P_2\lor\neg P_4\tab & (6,i,P_5) 
			\end{align*}
			\item \begin{align*}
				\neg P_1\lor\neg P_4\tab & (8,j,P_2)
			\end{align*}
			\item \begin{align*}
				\neg P_1\lor P_2\lor\neg P_5\tab & (1,k,P_4)
			\end{align*}
			\item \begin{align*}
				\neg P_1\lor P_2\lor\neg P_4\tab & (5, j,P_5)
			\end{align*}
			\item \begin{align*}
				P_2\lor P_3\lor\neg P_4\tab & (4,m,P_1)
			\end{align*}
			\item \begin{align*}
				\neg P_1\lor\neg P_4\lor P_5\tab & (3, o,P_3)
			\end{align*}
			\item \begin{align*}
				\neg P_1\lor\neg P_2\lor\neg P_4\tab (6,p,P_5)
			\end{align*}
			\item \begin{align*}
				\neg P_2\lor P_3\lor\neg P_4\tab & (4,p,P_1)
			\end{align*}
			\item \begin{align*}
				P_3\lor\neg P_4\tab & (8,q,P_2)
			\end{align*}
			\item \begin{align*}
				\neg P_1\lor\neg P_4\lor P_5\tab & (3,s,P_3) 
			\end{align*}
			\item \begin{align*}
				\neg P_1\lor\neg P_2\lor\neg P_4\tab & (6,t,P_5) 
			\end{align*}
		\end{enumerate}
	\end{multicols}
	\item $A=((P\to\neg R)\leftrightarrow(Q\land\neg P\land R))\to S.\tab P<Q<R<S$\\\\\emph{\textbf{Shannon}:}\\\begin{align*}
		A[1/P]&=((1\to\neg R)\leftrightarrow(Q\land\neg 1\land R))\to S=((1\to\neg R)\leftrightarrow0)\to S\\
		A[0/P]&=((0\to\neg R)\leftrightarrow(Q\land\neg 0\land R))\to S=(1\leftrightarrow(Q\land R))\to S\\
		A&=(P\Rightarrow A[1/P], A[0/P])\\
		A_{1}[1/Q]&=((1\to\neg R)\leftrightarrow(1\land\neg 1\land R))\to S=((1\to\neg R)\leftrightarrow0)\to S\\
		A_{1}[0/Q]&=((1\to\neg R)\leftrightarrow(0\land\neg 1\land R))\to S=((1\to\neg R)\leftrightarrow 0)\to S\\
		A_1&=(Q\Rightarrow A_1[1/Q], A_1[0/Q])\\
		A_{0}[1/Q]&=((0\to\neg R)\leftrightarrow(1\land\neg 0\land R))\to S=(1\leftrightarrow R)\to S \\
		A_{0}[0/Q]&=((0\to\neg R)\leftrightarrow(0\land\neg 0\land R))\to S=((0\to\neg R)\leftrightarrow0)\to S=1\\
		A_1&=(Q\Rightarrow A_1[1/Q], A_1[0/Q])\\
		A_{11}[1/R]&=((1\to\neg 1)\leftrightarrow(1\land\neg 1\land 1))\to S=S\\
		A_{11}[0/R]&=((1\to\neg 0)\leftrightarrow(1\land\neg 1\land 0))\to S=1\\
		A_{10}[1/R]&=((1\to\neg 1)\leftrightarrow(0\land\neg 1\land 1))\to S=S\\
		A_{10}[0/R]&=((1\to\neg 0)\leftrightarrow(0\land\neg 1\land 0))\to S=1\\
		A_{11}&=(R\Rightarrow A_{11}[1/R], A_{11}[0/R])\\
		A_{10}&=(R\Rightarrow A_{10}[1/R], A_{10}[0/R])\\
		A_{01}[1/R]&=((0\to\neg 1)\leftrightarrow(1\land\neg 0\land 1))\to S=S\\
		A_{01}[0/R]&=((0\to\neg 0)\leftrightarrow(1\land\neg 0\land 0))\to S=1\\
		A_{00}[1/R]&=((0\to\neg 1)\leftrightarrow(0\land\neg 0\land 1))\to S=1\\
		A_{00}[0/R]&=((0\to\neg 0)\leftrightarrow(0\land\neg 0\land 0))\to S=1\\
		A_{01}&=(R\Rightarrow A_{01}[1/R], A_{01}[0/R])\\
		A_{00}&=(R\Rightarrow A_{00}[1/R], A_{00}[0/R])\\
		A_{111}[1/S]&=1,\>A_{111}[0/S]=0,\>A_{110}[1/S]=1,\>A_{110}[0/S]=1\\
		A_{101}[1/S]&=1,\>A_{101}[0/S]=0,\>A_{100}[1/S]=1,\>A_{100}[0/S]=1\\
		A_{011}[1/S]&=1,\>A_{011}[0/S]=0,\>A_{010}[1/S]=1,\>A_{010}[0/S]=1\\
		A_{001}[1/S]&=1,\>A_{001}[0/S]=1,\>A_{000}[1/S]=1,\>A_{000}[0/S]=1
	\end{align*}
	\emph{\textbf{BDT}:}\\
	\begin{center}
		\begin{forest}
		BDT
		[P
			[Q
				[R
					[S
						[1][1]
					]
					[S
						[1][1]
					]
				]
				[R
					[S
						[1][1]
					]
					[S
						[0][1]
					]
				]
			]
			[Q
				[R
					[S
						[1][1]
					]
					[S
						[0][1]
					]
				]
				[R
					[S
						[1][1]
					]
					[S
						[0][1]
					]
				]
			]
		]
	\end{forest}
	\end{center}
	\emph{\textbf{ROBDD}:}\\
	\begin{center}
		\begin{forest}
			BDT
			[P
				[Q,
					tikz={\draw [ 0 my edge]  () [looseness=1.5, bend right=120] to (my one) ;}[,phantom]
					[R,
						tikz={\draw [ 0 my edge]  () [looseness=1.8, bend right=120] to (my one) ;}[,phantom]
						[S 
							[0, name = my zero] 
							[1, name = my one] 
						]
					]
				]
				[Q,
					[R,
						tikz={\draw [ 0 my edge] [bend right=10] () to (my one) ;}[,phantom]
						[S,
							tikz={\draw [ 0 my edge]  () [looseness=1.2, bend right=10] to (my zero) ;}
							tikz={\draw [ my edge] () [looseness=1.2, bend right=160] to (my one) ;}
							[,phantom]
						]
					]
					[R,
						tikz={\draw [ 0 my edge] [looseness=1.6, bend left=100] () to (my one) ;}[,phantom]
						[S,
							tikz={\draw [ my edge] () to (my one) ;}
							tikz={\draw [ 0 my edge] [looseness=.8, bend left=150] () to (my zero) ;}
							[,phantom]
						]
					]
				]
			]
		\end{forest}
		\begin{forest}
			BDT
			[P
				[Q,
					tikz={\draw [ 0 my edge]  () [looseness=1.5, bend right=120] to (my one) ;}[,phantom]
					[R,
						tikz={\draw [ 0 my edge]  () [looseness=1.8, bend right=120] to (my one) ;}[,phantom]
						[S 
							[0, name = my zero] 
							[1, name = my one] 
						]
					]
				]
				[Q,
					[R,
						tikz={\draw [ 0 my edge]  () [bend right=10] to (my one) ;}
						tikz={\draw [ my edge ] () [bend right] to (my);}
						[,phantom]
					]
					[R,		
						[S,
							tikz={\draw [ 0 my edge]  () [bend right=10] to (my zero) ;}[,phantom]
							tikz={\draw [my edge]  () [bend left=10] to (my one) ;}
							[,phantom],
							name = my
						]
					]
				]
			]
		\end{forest}
		\begin{forest}
			BDT
			[P
				[Q,
					tikz = {\draw [0 my edge] () [looseness=1.3, bend right=120] to (my one) ;}[,phantom]
					[R, name = myr,
						tikz = {\draw [0 my edge] () [looseness=1.3, bend right=120] to (my one) ;}[,phantom]
						[S, name = mys,
							[0, name = my zero] 
							[1, name = my one]
						]
					]
				]
				[Q,
					tikz = {\draw [0 my edge] () to (myr) ;}[,phantom]
					[R,
						tikz = {\draw [ 0 my edge] () [looseness=1.3, bend left=10] to (my one) ;}[,phantom]
						tikz = {\draw [my edge] [bend right] () to (mys) ;}
					]
				]
			]
		\end{forest}
	\end{center}
	\begin{align*}
		&\mathcal{T}(A)=\{P,Q,R,S\},\>|\mathcal{T(A)}|=4\\
		A:&\>\{\neg P,\neg Q,R,S\},\{\neg P,Q,R,S\},\>\{P,\neg Q,R,S\},\>\{P,Q,R,S\}\\
		(P\Rightarrow&(Q\Rightarrow1,(R\Rightarrow1,(S\Rightarrow1,0))),(Q\Rightarrow(R\Rightarrow1,(S\Rightarrow1,0)),(R\Rightarrow1,(S\Rightarrow1,0))))
	\end{align*}
	\begin{align*}
		=&(P\Rightarrow(Q\Rightarrow(R\Rightarrow(S\Rightarrow1,0))))&\textrm{ - ordered}\\
		=&(P\Rightarrow(Q\Rightarrow(R\Rightarrow(S\Rightarrow 1,0),(S\Rightarrow 1,0),(R\Rightarrow(S\Rightarrow 1,0),(S\Rightarrow 1,0))),\\&(Q\Rightarrow(R\Rightarrow(S\Rightarrow 1,0),(S\Rightarrow 1,0),(R\Rightarrow(S\Rightarrow 1,0),(S\Rightarrow 1,0))))&\textrm{ - full unordered}\\
		=&(P\Rightarrow(Q\Rightarrow1,(R\Rightarrow1,(S\Rightarrow1,0))))&\textrm{ - full ordered}
	\end{align*}
	\item 
	$A$ - Serhiy and Boris are about the same age, $B$ - Serhiy is older than Boris, $C$ - Nadiya and Boris are of different age, $D$ - Boris is older than Fedor
	\begin{align*}
		T&=(A\lor B)\land(A\to C)\land(B\to D)\land (C\to D)=\\&=(A\lor B)\land(\neg A\lor C)\land(\neg B\lor D)\land (\neg C\lor D)=\\&=(\neg A\lor C)\land(A\lor B)\land D
	\end{align*}
	$W=\{A\lor B,\neg A\lor C,\neg B\lor D,\neg C\lor D\}$
	\\\\\emph{\textbf{DPLL:}}\\
	\begin{itemize}
		\item [\textbf{SPLIT}] $(A)\\W_{11}=\{B,\neg B\lor D,\neg C\lor D\}\\W_{12}=\{C,\neg B\lor D,\neg C\lor D\}$
		\item [\textbf{UNIT}] $(B\in W_{11},C\in W_{12})\\W_{21}=\{D,\neg C\lor D\}\\W_{22}=\{\neg B\lor D,D\}$
		\item [\textbf{UNIT}] $(D\in W_{21},D\in W_{22})\\W_{31}=\{\neg C\}\\W_{32}=\{\neg B\}$
		\item [\textbf{UNIT}] $(C\in W_{21},B\in W_{22})\\W_{41}=\O\\W_{42}=\O$
	\end{itemize}
	W - unsatisfiable
	\\\\\emph{\textbf{Resolution:}}\\
	\begin{multicols}{4}
		\begin{enumerate}[(1)]
			\item $A\lor B$
			\item $\neg A\lor C$
			\item $\neg B\lor D$
			\item $\neg C\lor D$
		\end{enumerate}
	\end{multicols}
	\begin{multicols}{2}
		\begin{enumerate}
			\item \begin{align*}
				B\lor C\tab &(1,2,A)
			\end{align*}
			\item \begin{align*}
				\neg A\lor D\tab & (2,4,C) 
			\end{align*}
			\item \begin{align*}
				A\lor D\tab (1,3,B)
			\end{align*}
			\item \begin{align*}
				D\tab & (b,c,A)
			\end{align*}
		\end{enumerate}
	\end{multicols}
	\emph{\textbf{Shannon:}}\\\\
	$T=(A\lor B)\land(\neg A\lor C)\land(\neg B\lor D)\land (\neg C\lor D),\>A<B<C<D$
	\begin{align*}
		T[1/A]&=(1\lor B)\land(\neg 1\lor C)\land(\neg B\lor D)\land (\neg C\lor D)\\
		T[0/A]&=(0\lor B)\land(\neg 0\lor C)\land(\neg B\lor D)\land (\neg C\lor D)\\
		T&=(A\Rightarrow T[1/A],T[0/A])\\
		T_0[1/B]&=(1\lor 1)\land(\neg 1\lor C)\land(\neg 1\lor D)\land (\neg C\lor D)\\
		T_0[0/B]&=(1\lor 0)\land(\neg 1\lor C)\land(\neg 0\lor D)\land (\neg C\lor D)\\
		T_0&=(B\Rightarrow T_0[1/B],T_0[0/B])\\
		T_1[1/B]&=(0\lor 1)\land(\neg 0\lor C)\land(\neg 1\lor D)\land (\neg C\lor D)\\
		T_1[0/B]&=(0\lor 0)\land(\neg 0\lor C)\land(\neg 0\lor D)\land (\neg C\lor D)=0\\
		T_1&=(B\Rightarrow T_1[1/B],T_1[0/B])\\
		T_{00}[1/C]&=(1\lor 1)\land(\neg 1\lor 1)\land(\neg 1\lor D)\land (\neg 1\lor D)=D\\
		T_{00}[0/C]&=(1\lor 1)\land(\neg 1\lor 0)\land(\neg 1\lor D)\land (\neg 0\lor D)=0\\
		T_{01}[1/C]&=(1\lor 0)\land(\neg 1\lor 1)\land(\neg 0\lor D)\land (\neg 1\lor D)=D\\
		T_{01}[0/C]&=(1\lor 0)\land(\neg 1\lor 0)\land(\neg 0\lor D)\land (\neg 0\lor D)=0\\
		T_{00}&=(C\Rightarrow T_{00}[1/C],T_{00}[0/C])\\
		T_{01}&=(C\Rightarrow T_{01}[1/C],T_{01}[0/C])\\
		T_{10}[1/C]&=(0\lor 1)\land(\neg 0\lor 1)\land(\neg 1\lor D)\land (\neg 1\lor D)=D\\
		T_{10}[0/C]&=(0\lor 1)\land(\neg 0\lor 0)\land(\neg 1\lor D)\land (\neg 0\lor D)=D\\
		T_{11}[1/C]&=(0\lor 0)\land(\neg 0\lor 1)\land(\neg 0\lor D)\land (\neg 1\lor D)=0\\
		T_{11}[0/C]&=(0\lor 0)\land(\neg 0\lor 0)\land(\neg 0\lor D)\land (\neg 0\lor D)=0\\
		T_{10}&=(C\Rightarrow T_{10}[1/C],T_{10}[0/C])\\
		T_{11}&=(C\Rightarrow T_{11}[1/C],T_{11}[0/C])
	\end{align*}
	\begin{align*}
		T_{000}[1/D]&=1,\>T_{000}[0/D]=0,\>T_{001}[1/D]=0,\>T_{001}[0/D]=0\\
		T_{010}[1/D]&=1,\>T_{010}[0/D]=0,\>T_{011}[1/D]=0,\>T_{011}[0/D]=0\\
		T_{100}[1/D]&=1,\>T_{100}[0/D]=0,\>T_{101}[1/D]=1,\>T_{101}[0/D]=0\\
		T_{101}[1/D]&=0,\>T_{101}[0/D]=0,\>T_{111}[1/D]=0,\>T_{101}[0/D]=0\\
	\end{align*}
\end{enumerate}




































\end{document}